specs/Spec.Blake2s.fst
@@ -149,20 +149,25 @@ let blake2_compress h m offset flag =
   h
 
 
-val blake2s_internal : dd:size_nat{0 < dd /\ dd * bytes_in_block <= max_size_t}  -> d:lbytes (dd * bytes_in_block) -> ll:size_nat -> kk:size_nat{kk<=32} -> nn:size_nat{1 <= nn /\ nn <= 32} -> Tot (lbytes nn)
-
-let blake2s_internal dd d ll kk nn =
-  let h = const_init in
+val blake2s_internal1 : h:intseq U32 8 -> kk:size_nat{kk<=32} -> nn:size_nat{1 <= nn /\ nn <= 32} -> Tot (intseq U32 8)
+let blake2s_internal1 h kk nn =
   let h = h.[0] <- h.[0] ^. (u32 0x01010000) ^. ((u32 kk) <<. (u32 8)) ^. (u32 nn) in
-  let h =
-    if dd > 1 then
-    repeati (dd - 1) (fun i h ->
-	   let to_compress : intseq U32 16 =
-	   uints_from_bytes_le (sub d (i*bytes_in_block) bytes_in_block) in
-	   blake2_compress h to_compress (u64 ((i+1)*block_bytes)) false
-    ) h else h
-  in
-  let offset : size_nat = (dd-1)*16*4 in
+  h
+
+val blake2s_internal2 : h:intseq U32 8 -> dd:size_nat{0 < dd /\ dd * bytes_in_block <= max_size_t} -> d:lbytes (dd * bytes_in_block) -> Tot (h:intseq U32 8)
+let blake2s_internal2 h dd d =
+  if dd > 1 then
+  repeati (dd - 1) (fun i h ->
+	 let to_compress : intseq U32 16 =
+	 uints_from_bytes_le (sub d (i * bytes_in_block) bytes_in_block) in
+    blake2_compress h to_compress (u64 ((i + 1) * block_bytes)) false
+  ) h else h
+
+
+val blake2s_internal3 : h:intseq U32 8 -> dd:size_nat{0 < dd /\ dd * bytes_in_block <= max_size_t} -> d:lbytes (dd * bytes_in_block) -> ll:size_nat -> kk:size_nat{kk<=32} -> nn:size_nat{1 <= nn /\ nn <= 32} -> Tot (lbytes nn)
+
+let blake2s_internal3 h dd d ll kk nn =
+  let offset : size_nat = (dd - 1) * 16 * 4 in
   let last_block : intseq U32 16 = uints_from_bytes_le (sub d offset bytes_in_block) in
   let h =
     if kk = 0 then
@@ -172,6 +177,14 @@ let blake2s_internal dd d ll kk nn =
   in
   sub (uints_to_bytes_le h) 0 nn
 
+
+val blake2s_internal : dd:size_nat{0 < dd /\ dd * bytes_in_block <= max_size_t} -> d:lbytes (dd * bytes_in_block) -> ll:size_nat -> kk:size_nat{kk<=32} -> nn:size_nat{1 <= nn /\ nn <= 32} -> Tot (lbytes nn)
+let blake2s_internal dd d ll kk nn =
+  let h = const_init in
+  let h = blake2s_internal1 h kk nn in
+  let h = blake2s_internal2 h dd d in
+  let k = blake2s_internal3 h dd d ll kk nn in
+  k
 
 val blake2s : ll:size_nat{0 < ll /\ ll <= max_size_t - 2 * bytes_in_block } ->  d:lbytes ll ->  kk:size_nat{kk<=32} -> k:lbytes kk -> nn:size_nat{1 <= nn /\ nn <= 32} -> Tot (lbytes nn)
 
